a basic version of union marshalling

lib/Marshalling/UnionMarshalling.i.dfy
@@ -9,15 +9,13 @@ refines Marshalling {
   
   import TGM = IntegerMarshalling(TagInt)
 
-  datatype UnionType = 
-    | Left(l : CaseMarshalling0.UnmarshalledType)
-    | Right(r: CaseMarshalling1.UnmarshalledType)
+  datatype UnmarshalledType = 
+    | Case0(l : CaseMarshalling0.UnmarshalledType)
+    | Case1(r: CaseMarshalling1.UnmarshalledType)
 
   datatype Config = Config(tgmCfg: TGM.Config,
     elemCfg0: CaseMarshalling0.Config,
     elemCfg1: CaseMarshalling1.Config)
-
-  type UnmarshalledType = UnionType
 
   type TagType = TGM.UnmarshalledType
 
@@ -48,8 +46,8 @@ refines Marshalling {
     var tagEnd := getTagEnd() as int;
     var tag := TGM.parse(cfg.tgmCfg, data[..tagEnd]);
 
-    if tag == 0 then Left(CaseMarshalling0.parse(cfg.elemCfg0, data[tagEnd..]))
-      else Right(CaseMarshalling1.parse(cfg.elemCfg1, data[tagEnd..]))
+    if tag == 0 then Case0(CaseMarshalling0.parse(cfg.elemCfg0, data[tagEnd..]))
+      else Case1(CaseMarshalling1.parse(cfg.elemCfg1, data[tagEnd..]))
   }
 
   method TryParse(cfg: Config, data: mseq<byte>) returns (ovalue: Option<UnmarshalledType>)
@@ -66,10 +64,10 @@ refines Marshalling {
 
     if tag == 0 {
       var left :- CaseMarshalling0.TryParse(cfg.elemCfg0, data[tagEnd..]);
-      ovalue := Some(Left(left));
+      ovalue := Some(Case0(left));
     } else {
       var right :- CaseMarshalling1.TryParse(cfg.elemCfg1, data[tagEnd..]);
-      ovalue := Some(Right(right));
+      ovalue := Some(Case1(right));
     }
   }
 
@@ -106,10 +104,10 @@ refines Marshalling {
 
     if tag == 0 {
       var leftValue := CaseMarshalling0.Parse(cfg.elemCfg0, data[tagEnd..]);
-      return Left(leftValue);
+      return Case0(leftValue);
     } else {
       var rightValue := CaseMarshalling1.Parse(cfg.elemCfg1, data[tagEnd..]);
-      return Right(rightValue);
+      return Case1(rightValue);
     }
   }
 
@@ -117,10 +115,10 @@ refines Marshalling {
   {
     && TagInt.MinValue() <= 0 < 1 < TagInt.UpperBound()
     && match value {
-      case Left(leftValue) =>
+      case Case0(leftValue) =>
         (&& CaseMarshalling0.marshallable(cfg.elemCfg0, leftValue)
         && getTagEnd() as nat + CaseMarshalling0.size(cfg.elemCfg0, leftValue) as nat < Uint64UpperBound())
-      case Right(rightValue) =>
+      case Case1(rightValue) =>
         (&& CaseMarshalling1.marshallable(cfg.elemCfg1, rightValue)
         && getTagEnd() as nat + CaseMarshalling1.size(cfg.elemCfg1, rightValue) as nat < Uint64UpperBound())
     }
@@ -130,8 +128,8 @@ refines Marshalling {
   {
     var tagEnd := getTagEnd();
     match value {
-      case Left(leftValue) => tagEnd + CaseMarshalling0.size(cfg.elemCfg0, leftValue)
-      case Right(rightValue) => tagEnd + CaseMarshalling1.size(cfg.elemCfg1, rightValue)
+      case Case0(leftValue) => tagEnd + CaseMarshalling0.size(cfg.elemCfg0, leftValue)
+      case Case1(rightValue) => tagEnd + CaseMarshalling1.size(cfg.elemCfg1, rightValue)
     }
   }
 
@@ -139,11 +137,11 @@ refines Marshalling {
   {
     sz := getTagEnd();
     match value {
-      case Left(leftValue) => {
+      case Case0(leftValue) => {
         var leftSize := CaseMarshalling0.Size(cfg.elemCfg0, leftValue);
         sz := sz + leftSize;
       }
-      case Right(rightValue) => {
+      case Case1(rightValue) => {
         var rightSize := CaseMarshalling1.Size(cfg.elemCfg1, rightValue);
         sz := sz + rightSize;
       }
@@ -156,7 +154,7 @@ refines Marshalling {
     ghost var tagEnd : uint64 := getTagEnd();
 
     match value
-    case Left(leftValue) => {
+    case Case0(leftValue) => {
       end := TGM.Marshall(cfg.tgmCfg, 0, inout data, start);
       ghost var newdata1 :seq<byte>, end1 := data, end;
       end := CaseMarshalling0.Marshall(cfg.elemCfg0, leftValue, inout data, end);
@@ -164,7 +162,7 @@ refines Marshalling {
       assert newdata1[start..end1] == data[start..end1];
       assert data[start..end][..tagEnd] == data[start..end1];
     }
-    case Right(rightValue) => {
+    case Case1(rightValue) => {
       end := TGM.Marshall(cfg.tgmCfg, 1, inout data, start);
       ghost var newdata1 :seq<byte>, end1 := data, end;
       end := CaseMarshalling0.Marshall(cfg.elemCfg1, rightValue, inout data, end);
@@ -173,214 +171,18 @@ refines Marshalling {
       assert data[start..end][..tagEnd] == data[start..end1];
     }
   }
+
+  predicate settable(cfg: Config, slice: Slice, data: mseq<byte>, value: UnmarshalledType)
+  {
+    && validConfig(cfg)
+    && marshallable(cfg, value)
+    && slice.WF'(data)
+    && size(cfg, value) <= |slice|
+  }
+
+  // method Set(cfg: Config, slice: Slice, linear inout data: mseq<byte>, value: UnmarshalledType)
+  //   requires settable(cfg, slice, old_data, value)
+  // {
+
+  // }
 }
-
-// abstract module Union3Marshalling refines Marshalling {
-//   import CaseMarshalling0 : Marshalling
-//   import CaseMarshalling1 : Marshalling
-//   import CaseMarshalling2 : Marshalling
-//   import TGM : IntegerMarshalling
-//   // import Sequences
-
-//   datatype UnionType = 
-//     | Case0(c0: CaseMarshalling0.UnmarshalledType)
-//     | Case1(c1: CaseMarshalling1.UnmarshalledType)
-//     | Case2(c2: CaseMarshalling2.UnmarshalledType)
-
-//   type UnmarshalledType = UnionType
-
-//   type TagType = TGM.UnmarshalledType
-
-//   function method getTagEnd(): uint64
-//   {
-//     TGM.Int.Size() as uint64
-//   }
-
-//   predicate parsable(data: mseq<byte>)
-//   {
-//     var tagEnd := getTagEnd() as int;
-//     && |data| >= tagEnd
-//     && TGM.parsable(data[..tagEnd])
-//     && TGM.Int.fitsInUint64(TGM.parse(data[..tagEnd]))
-//     && var tag := TGM.Int.toInt(TGM.parse(data[..tagEnd]));
-//     (if tag == 0 then CaseMarshalling0.parsable(data[tagEnd..])
-//       else if tag == 1 then CaseMarshalling1.parsable(data[tagEnd..])
-//       else CaseMarshalling2.parsable(data[tagEnd..]))
-//   }
-
-//   function parse(data: mseq<byte>) : UnmarshalledType
-//   {
-//     var tagEnd := getTagEnd() as int;
-//     var tag := TGM.Int.toInt(TGM.parse(data[..tagEnd]));
-
-//     if tag == 0 then Case0(CaseMarshalling0.parse(data[tagEnd..]))
-//       else if tag == 1 then Case1(CaseMarshalling1.parse(data[tagEnd..]))
-//       else Case2(CaseMarshalling2.parse(data[tagEnd..]))
-//   }
-
-//   method TryParse(data: mseq<byte>) returns (ovalue: Option<UnmarshalledType>)
-//   {
-//     var tagEnd := getTagEnd();
-
-//     if tagEnd > |data| as uint64 {
-//       return None;
-//     }
-
-//     var tagOvalue := TGM.TryParse(data[..tagEnd]);
-    
-//     if tagOvalue.None? {
-//       return None;
-//     }
-
-//     if !TGM.Int.fitsInUint64(tagOvalue.value) {
-//       return None;
-//     }
-
-//     var tag := TGM.Int.toUint64(tagOvalue.value);
-//     ovalue := None;
-
-//     if tag == 0 {
-//       var valueOpt := CaseMarshalling0.TryParse(data[tagEnd..]);
-//       if valueOpt.Some? {
-//         ovalue := Some(Case0(valueOpt.value));
-//       }
-//     } else if tag == 1 {
-//       var valueOpt := CaseMarshalling1.TryParse(data[tagEnd..]);
-//       if valueOpt.Some? {
-//         ovalue := Some(Case1(valueOpt.value));
-//       }
-//     } else {
-//       var valueOpt := CaseMarshalling2.TryParse(data[tagEnd..]);
-//       if valueOpt.Some? {
-//         ovalue := Some(Case2(valueOpt.value));
-//       }
-//     }
-//   }
-
-//   method Parsable(data: mseq<byte>) returns (p: bool)
-//   {
-//     var tagEnd := getTagEnd();
-
-//     if tagEnd > |data| as uint64 {
-//       return false;
-//     }
-
-//     var tagOvalue := TGM.TryParse(data[..tagEnd]);
-    
-//     if tagOvalue.None? {
-//       return false;
-//     }
-
-//     if !TGM.Int.fitsInUint64(tagOvalue.value) {
-//       return false;
-//     }
-
-//     var tag := TGM.Int.toUint64(tagOvalue.value);
-
-//     if tag == 0 {
-//       p := CaseMarshalling0.Parsable(data[tagEnd..]);
-//     } else if tag == 1{
-//       p := CaseMarshalling1.Parsable(data[tagEnd..]);
-//     } else {
-//       p := CaseMarshalling2.Parsable(data[tagEnd..]);
-//     }
-//   }
-
-//   method Parse(data: mseq<byte>) returns (value: UnmarshalledType)
-//   {
-//     var tagEnd := getTagEnd();
-//     var tagOvalue := TGM.TryParse(data[..tagEnd]);
-//     var tag := TGM.Int.toUint64(tagOvalue.value);
-
-//     if tag == 0 {
-//       var val := CaseMarshalling0.Parse(data[tagEnd..]);
-//       value := Case0(val);
-//     } else if tag == 1 {
-//       var val := CaseMarshalling1.Parse(data[tagEnd..]);
-//       value := Case1(val);
-//     } else {
-//       var val := CaseMarshalling2.Parse(data[tagEnd..]);
-//       value := Case2(val);    
-//     }
-//   }
-
-//   predicate marshallable(value: UnmarshalledType)
-//   {
-//     && TGM.Int.MinValue() <= 0 < 2 < TGM.Int.UpperBound()
-//     && match value {
-//       case Case0(c0) => CaseMarshalling0.marshallable(c0)
-//       case Case1(c1) => CaseMarshalling1.marshallable(c1)
-//       case Case2(c2) => CaseMarshalling2.marshallable(c2)
-//     }
-//   }
-
-//   function size(value: UnmarshalledType) : nat
-//   {
-//     var tagEnd := getTagEnd();
-//     match value {
-//       case Case0(c0) => tagEnd as nat + CaseMarshalling0.size(c0)
-//       case Case1(c1) => tagEnd as nat + CaseMarshalling1.size(c1)
-//       case Case2(c2) => tagEnd as nat + CaseMarshalling2.size(c2)
-//     }
-//   }
-
-//   method Size(value: UnmarshalledType) returns (sz: uint64)
-//   {
-//     sz := getTagEnd();
-//     match value
-//     case Case0(c0) => {
-//       var size := CaseMarshalling0.Size(c0);
-//       sz := sz + size;
-//     }
-//     case Case1(c1) => {
-//       var size := CaseMarshalling1.Size(c1);
-//       sz := sz + size;
-//     }
-//     case Case2(c2) => {
-//       var size := CaseMarshalling2.Size(c2);
-//       sz := sz + size;
-//     }
-//   }
-
-//   method Marshall(value: UnmarshalledType, linear data: mseq<byte>, start: uint64)
-//     returns (linear newdata: mseq<byte>, end: uint64)
-//   {
-//     ghost var tagEnd : uint64 := getTagEnd();
-
-//     match value
-//     case Case0(c0) => {
-//       newdata, end := TGM.Marshall(TGM.Int.fromUint64(0), data, start);
-//       ghost var newdata1 :seq<byte>, end1 := newdata, end;
-//       newdata, end := CaseMarshalling0.Marshall(c0, newdata, end);
-
-//       assert newdata[start..end][..tagEnd] == newdata1[start..end1] == newdata[start..end1];
-//       ghost var tag := TGM.Int.toInt(TGM.parse(newdata[start..end1]));
-//       TGM.Int.fromtoInverses();
-//       assert tag == 0;
-//     }
-//     case Case1(c1) => {
-//       newdata, end := TGM.Marshall(TGM.Int.fromUint64(1), data, start);
-//       ghost var newdata1 :seq<byte>, end1 := newdata, end;
-//       newdata, end := CaseMarshalling1.Marshall(c1, newdata, end);
-  
-//       assert newdata1[start..end1] == newdata[start..end1];
-//       ghost var tag := TGM.Int.toInt(TGM.parse(newdata[start..end1]));
-//       TGM.Int.fromtoInverses();
-//       assert tag == 1;
-
-//       assert newdata[start..end][..tagEnd] == newdata[start..end1];
-//     }
-//     case Case2(c2) => {
-//       newdata, end := TGM.Marshall(TGM.Int.fromUint64(2), data, start);
-//       ghost var newdata1 :seq<byte>, end1 := newdata, end;
-//       newdata, end := CaseMarshalling2.Marshall(c2, newdata, end);
-  
-//       assert newdata1[start..end1] == newdata[start..end1];
-//       ghost var tag := TGM.Int.toInt(TGM.parse(newdata[start..end1]));
-//       TGM.Int.fromtoInverses();
-//       assert tag == 2;
-
-//       assert newdata[start..end][..tagEnd] == newdata[start..end1];
-//     }
-//   }
-// }
